share/steel/examples/pulse/dice/common/HashTable.fst
@@ -5,18 +5,48 @@ open FStar.Ghost
 open Steel.ST.Util
 open Steel.FractionalPermission
 module R = Steel.ST.Reference
+module A = Steel.ST.Array
 module L = Steel.ST.SpinLock
 module US = FStar.SizeT
 module U32 = FStar.UInt32
 
 // Hash table types 
 
-assume val ht_t : Type0
+noeq
+type cell (kt vt : Type) =
+  | Clean
+  | Zombie
+  | Used : k:kt -> v:vt -> cell kt vt
 
-type ht_ref_t = r:R.ref ht_t & L.lock (exists_ (fun ht -> R.pts_to r full_perm ht))
+noeq
+type ht_sig = {
+  sz : pos;
+  kt : eqtype;
+  vt : Type;
+  hashf : kt -> nat;
+}
 
-assume val new_table (_:unit) : ht_t
+let mk_ht_sig sz kt vt hashf = { sz; kt; vt; hashf }
+
+noeq
+type ht_t (s:ht_sig) = {
+  contents : A.larray (cell s.kt s.vt) s.sz;
+}
+
+type ht_ref_t (s:ht_sig) = r:R.ref (ht_t s) & L.lock (exists_ (fun ht -> R.pts_to r full_perm ht))
+
+// Hash table interface
+
+assume val new_table (#s:ht_sig) : ht_t s
+
+assume val store (#s:ht_sig) (ht:ht_t s) (k:s.kt) (v:s.vt) : unit
+
+assume val get (#s:ht_sig) (ht:ht_t s) (k:s.kt) : s.vt
+
+assume val delete (#s:ht_sig) (ht:ht_t s) (k:s.kt) : unit
+
+assume val destroy (#s:ht_sig) (ht:ht_t s) : unit
 
 // Session ID types
 
-type sid_ref_t = r:R.ref US.t & L.lock (exists_ (fun n -> R.pts_to r full_perm n))
+type sid_ref_t = r:R.ref nat & L.lock (exists_ (fun n -> R.pts_to r full_perm n))
